run allows a state machine to end early

core/Core.v
@@ -129,21 +129,57 @@ Module ByteListReader : READER.
   (* state machines *)
 
   Fixpoint run {S A}
-           (f : state_machine S A) (s : S) (l : list byte) : fold_state S (A * list byte) :=
+           (f : S -> state_machine S A + A) (s : S) (l : list byte) : fold_state S (A * list byte) :=
     match l with
     | [] => More s
-    | b :: l => match f b s with
-                | Done a => Done (a, l)
-                | More s => run f s l
-                | Error => Error
+    | b :: l => match f s with
+                | inl m => match m b s with
+                           | Done a => Done (a, l)
+                           | More s => run f s l
+                           | Error => Error
+                           end
+                | inr a => Done (a, b :: l)
                 end
     end.
 
   Definition fold {S A} (f : state_machine S A) (s : S) (l : list byte) :=
+    match run (fun _ => inl f) s l with
+    | Done (a, l) => Some (a, l)
+    | _ => None
+    end.
+
+  Definition fold_general {S A} (f : S -> state_machine S A + A) (s : S) (l : list byte) :=
     match run f s l with
     | Done (a, l) => Some (a, l)
     | _ => None
     end.
+
+  Lemma fold_general_unwrap : forall {S A : Type}
+                                     (f : S -> state_machine S A + A) (s : S) l,
+      unwrap (fold_general f s) l =
+      match l with
+      | [] => None
+      | b :: l => match f s with
+                | inl m => match m b s with
+                           | Done a => Some (a, l)
+                           | More s => unwrap (fold_general f s) l
+                           | Error => None
+                           end
+                | inr a => Some (a, b :: l)
+                end
+      end.
+  Proof.
+    intros.
+    unfold fold_general.
+    destruct l;
+      unfold unwrap.
+    - reflexivity.
+    - simpl.
+      destruct (f s).
+      + destruct (s0 b s);
+        reflexivity.
+      + reflexivity.
+  Qed.
 
   Lemma run_append :
     forall {S A : Type}  l1 l2 f (s : S),
@@ -159,9 +195,11 @@ Module ByteListReader : READER.
       reflexivity.
     - intros.
       simpl.
-      destruct (f a s); try reflexivity.
-      rewrite IHl1.
-      reflexivity.
+      destruct (f s).
+      + destruct (s0 a s); try reflexivity.
+        rewrite IHl1.
+        reflexivity.
+      + reflexivity.
   Qed.
 
   Definition one : state_machine unit byte :=
@@ -199,8 +237,8 @@ Module ByteListReader : READER.
   Lemma run_pair_inr : forall S1 A S2 B
                                (a : state_machine S1 A) (b : state_machine S2 B)
                                x bytes s,
-       run (pair a b) (inr (x, s)) bytes =
-      match run b s bytes with
+       run (fun _ => inl (pair a b)) (inr (x, s)) bytes =
+      match run (fun _ => inl b) s bytes with
       | Done (y, l)  => Done ((x, y), l)
       | More s => More (inr (x, s))
       | Error => Error
@@ -238,9 +276,9 @@ Module ByteListReader : READER.
   Lemma run_pair_inl : forall S1 A S2 B
                                (a : state_machine S1 A) (b : state_machine S2 B)
                                bytes s1 s2,
-      run (pair a b) (inl (s1, s2)) bytes =
-      match run a s1 bytes with
-      | Done (x, l) => run (pair a b) (inr (x, s2)) l
+      run (fun _ => inl (pair a b)) (inl (s1, s2)) bytes =
+      match run (fun _ => inl a) s1 bytes with
+      | Done (x, l) => run (fun _ => inl (pair a b)) (inr (x, s2)) l
       | More s1 => More (inl (s1, s2))
       | Error => Error
       end.
@@ -294,9 +332,9 @@ Module ByteListReader : READER.
                                   (a : state_machine S1 A)
                                   (b : state_machine S2 B)
                                   bytes f s,
-      run (sequence a b) (inl (s, f)) bytes =
-      match run a s bytes with
-      | Done (x, bytes) => run (sequence a b) (inr (f x)) bytes
+      run (fun _ => inl (sequence a b)) (inl (s, f)) bytes =
+      match run (fun _ => inl a) s bytes with
+      | Done (x, bytes) => run (fun _ => inl (sequence a b)) (inr (f x)) bytes
       | More s1 => More (inl (s1, f))
       | Error => Error
       end.
@@ -314,11 +352,11 @@ Module ByteListReader : READER.
                                   (a : state_machine S1 A)
                                   (b : state_machine S2 B)
                                   bytes s,
-      run (sequence a b) (inr s) bytes = match (run b s) bytes with
-                                         | Done (x, l) => Done (x, l)
-                                         | More s2 => More (inr s2)
-                                         | Error => Error
-                                         end.
+      run (fun _ => inl (sequence a b)) (inr s) bytes = match (run (fun _ => inl b) s) bytes with
+                                                        | Done (x, l) => Done (x, l)
+                                                        | More s2 => More (inr s2)
+                                                        | Error => Error
+                                                        end.
   Proof.
     unfold unwrap.
     induction bytes; simpl; intros.
@@ -398,8 +436,6 @@ Module ByteListReader : READER.
       simpl.
       now destruct (f b s).
   Qed.
-
-
 End ByteListReader.
 Arguments ByteListReader.error {_}.
 
